fstar/MLS.Test.FromExt.Encryption.fst
@@ -24,8 +24,8 @@ let normalize_text s =
     else
       failwith "normalize_text: don't start with 02"
 
-val test_leaf_generation: {|crypto_bytes bytes|} -> l:nat -> n:tree_size l -> i:leaf_index n -> bytes -> bytes -> ratchet_state bytes -> encryption_leaf_generation_test -> ML (bool & ratchet_state bytes)
-let test_leaf_generation #cb l n i encryption_secret sender_data_secret r_state test =
+val test_leaf_generation: {|crypto_bytes bytes|} -> l:nat -> i:leaf_index l -> bytes -> bytes -> ratchet_state bytes -> encryption_leaf_generation_test -> ML (bool & ratchet_state bytes)
+let test_leaf_generation #cb l i encryption_secret sender_data_secret r_state test =
   let r_output = extract_result (ratchet_get_key r_state) in
   let r_next_state = extract_result (ratchet_next_state r_state) in
   let key_ok = check_equal "key" bytes_to_hex_string (hex_string_to_bytes test.key) r_output.key in
@@ -37,42 +37,42 @@ let test_leaf_generation #cb l n i encryption_secret sender_data_secret r_state 
   let message_plaintext = extract_result (network_to_message_plaintext message_plaintext_network) in
   let message_ciphertext = extract_result (network_to_message_ciphertext message_ciphertext_network) in
   let message_1 = message_plaintext_to_message message_plaintext in
-  let message_2 = extract_result (message_ciphertext_to_message l n encryption_secret sender_data_secret message_ciphertext) in
+  let message_2 = extract_result (message_ciphertext_to_message l encryption_secret sender_data_secret message_ciphertext) in
   let message_2 = (({ (fst message_2) with wire_format = WF_mls_plaintext ()} <: message_content bytes), snd message_2) in
   let plaintext_eq_ciphertext_ok = test_equality message_1 message_2 in
   let sender_ok = MLS.TreeDEM.Message.Types.S_member? (fst message_1).sender in
   (key_ok && nonce_ok && plaintext_eq_ciphertext_ok && sender_ok, r_next_state)
 
-val test_leaf_generations: {|crypto_bytes bytes|} -> l:nat -> n:tree_size l -> i:leaf_index n -> bytes -> bytes -> ratchet_state bytes -> list encryption_leaf_generation_test -> ML bool
-let rec test_leaf_generations #cb l n i encryption_secret sender_data_secret r_state tests =
+val test_leaf_generations: {|crypto_bytes bytes|} -> l:nat -> i:leaf_index l -> bytes -> bytes -> ratchet_state bytes -> list encryption_leaf_generation_test -> ML bool
+let rec test_leaf_generations #cb l i encryption_secret sender_data_secret r_state tests =
   match tests with
   | [] -> true
   | h::t ->
-    let (head_ok, r_next_state) = test_leaf_generation l n i encryption_secret sender_data_secret r_state h in
-    let tail_ok = test_leaf_generations l n i encryption_secret sender_data_secret r_next_state t in
+    let (head_ok, r_next_state) = test_leaf_generation l i encryption_secret sender_data_secret r_state h in
+    let tail_ok = test_leaf_generations l i encryption_secret sender_data_secret r_next_state t in
     head_ok && tail_ok
 
-val test_leaf: {|crypto_bytes bytes|} -> l:nat -> n:tree_size l -> i:leaf_index n -> bytes -> bytes -> encryption_leaf_test -> ML bool
-let test_leaf #cb l n i encryption_secret sender_data_secret test =
-  let leaf_encryption_secret = extract_result (leaf_kdf n encryption_secret i) in
+val test_leaf: {|crypto_bytes bytes|} -> l:nat -> i:leaf_index l -> bytes -> bytes -> encryption_leaf_test -> ML bool
+let test_leaf #cb l i encryption_secret sender_data_secret test =
+  let leaf_encryption_secret = extract_result (leaf_kdf encryption_secret i) in
   let handshake_ratchet = extract_result (init_handshake_ratchet leaf_encryption_secret) in
   let application_ratchet = extract_result (init_application_ratchet leaf_encryption_secret) in
-  let handshake_ok = test_leaf_generations l n i encryption_secret sender_data_secret handshake_ratchet test.handshake in
-  let application_ok = test_leaf_generations l n i encryption_secret sender_data_secret application_ratchet test.application in
+  let handshake_ok = test_leaf_generations l i encryption_secret sender_data_secret handshake_ratchet test.handshake in
+  let application_ok = test_leaf_generations l i encryption_secret sender_data_secret application_ratchet test.application in
   handshake_ok && application_ok
 
-val test_leaves_aux: {|crypto_bytes bytes|} -> l:nat -> n:tree_size l -> bytes -> bytes -> leaf_tests:list encryption_leaf_test -> i:nat{i + List.Tot.length leaf_tests <= n} -> ML bool
-let rec test_leaves_aux #cb l n encryption_secret sender_data_secret leaf_tests i =
+val test_leaves_aux: {|crypto_bytes bytes|} -> l:nat -> bytes -> bytes -> leaf_tests:list encryption_leaf_test -> i:nat{i + List.Tot.length leaf_tests <= pow2 l} -> ML bool
+let rec test_leaves_aux #cb l encryption_secret sender_data_secret leaf_tests i =
   match leaf_tests with
   | [] -> true
   | h::t ->
-    let head_ok = test_leaf l n i encryption_secret sender_data_secret h in
-    let tail_ok = test_leaves_aux l n encryption_secret sender_data_secret t (i+1) in
+    let head_ok = test_leaf l i encryption_secret sender_data_secret h in
+    let tail_ok = test_leaves_aux l encryption_secret sender_data_secret t (i+1) in
     head_ok && tail_ok
 
-val test_leaves: {|crypto_bytes bytes|} -> l:nat -> n:tree_size l -> bytes -> bytes -> leaf_tests:list encryption_leaf_test{List.Tot.length leaf_tests <= n} -> ML bool
-let test_leaves #cb l n encryption_secret sender_data_secret leaf_tests =
-  test_leaves_aux l n encryption_secret sender_data_secret leaf_tests 0
+val test_leaves: {|crypto_bytes bytes|} -> l:nat -> bytes -> bytes -> leaf_tests:list encryption_leaf_test{List.Tot.length leaf_tests <= pow2 l} -> ML bool
+let test_leaves #cb l encryption_secret sender_data_secret leaf_tests =
+  test_leaves_aux l encryption_secret sender_data_secret leaf_tests 0
 
 val test_encryption_one: encryption_test -> ML bool
 let test_encryption_one t =
@@ -92,11 +92,11 @@ let test_encryption_one t =
     | Success cs -> begin
       let cb = mk_concrete_crypto_bytes cs in
       let n_leaves = UInt32.v t.n_leaves in
-      let n_nodes = n_leaves + n_leaves - 1 in
-      let l = if n_nodes > 0 then (MLS.TreeMath.Internal.log2 n_nodes) + 1 else failwith "there cannot be 0 leaves!" in
+      let l = if n_leaves > 0 then MLS.TreeMath.Internal.log2 n_leaves else failwith "there cannot be 0 leaves!" in
+      if pow2 l <> n_leaves then failwith "n_leaves is not a power of two!" else ();
       let leaves_ok =
         if List.Tot.length t.leaves <= n_leaves then
-          test_leaves #cb l n_leaves (hex_string_to_bytes t.encryption_secret) (hex_string_to_bytes t.sender_data_secret) t.leaves
+          test_leaves #cb l (hex_string_to_bytes t.encryption_secret) (hex_string_to_bytes t.sender_data_secret) t.leaves
         else
           failwith "list leaves is too big!"
       in
