fstar/MLS.Tree.fst
@@ -2,44 +2,40 @@ module MLS.Tree
 
 open MLS.Result
 
-let tree_size (l:nat) = n:pos{n <= pow2 l}
-let leaf_index (n:nat) = x:nat{x < n}
+let leaf_index (l:nat) = x:nat{x < pow2 l}
 
-type tree (l:nat) (n:tree_size l) (leaf_t:Type) (node_t:Type)=
- | TLeaf: data:leaf_t{l=0 /\ n=1} -> tree l n leaf_t node_t
- | TSkip: squash (l>0 /\ n <= pow2 (l-1)) -> tree (l-1) n leaf_t node_t -> tree l n leaf_t node_t
- | TNode: data:node_t{l>0 /\ pow2 (l-1) < n} -> left:tree (l-1) (pow2 (l-1)) leaf_t node_t -> right:tree (l-1) (n-pow2 (l-1)) leaf_t node_t -> tree l n leaf_t node_t
+type tree (l:nat) (leaf_t:Type) (node_t:Type)=
+ | TLeaf: data:leaf_t{l=0} -> tree l leaf_t node_t
+ | TNode: data:node_t{l>0} -> left:tree (l-1) leaf_t node_t -> right:tree (l-1) leaf_t node_t -> tree l leaf_t node_t
 
-type path (l:nat) (n:tree_size l) (i:leaf_index n) (leaf_t:Type) (node_t:Type) =
-  | PLeaf: data:leaf_t{l=0 /\ n=1 /\ i=0} -> path l n i leaf_t node_t
-  | PSkip: squash (l>0 /\ n <= pow2 (l-1)) -> path (l-1) n i leaf_t node_t -> path l n i leaf_t node_t
-  | PNode: data:node_t{l>0 /\ pow2 (l-1) < n} -> next:path (l-1) (if i < pow2 (l-1) then pow2 (l-1) else n-pow2 (l-1)) (if i < pow2 (l-1) then i else i-pow2 (l-1)) leaf_t node_t -> path l n i leaf_t node_t
+type path (l:nat) (leaf_t:Type) (node_t:Type) =
+  | PLeaf: data:leaf_t{l=0} -> path l leaf_t node_t
+  | PNode: data:node_t{l>0} -> next:path (l-1) leaf_t node_t -> path l leaf_t node_t
 
 type direction = | Left | Right
 
-let child_index (#n:nat) (l:pos{pow2 (l-1) < n}) (i:leaf_index n) : (dir:direction & (leaf_index (if dir = Left then (pow2 (l-1)) else (n-pow2 (l-1))))) =
-  if i < pow2 (l - 1) then (|Left, i|) else (|Right, i-pow2 (l-1)|)
-val order_subtrees: #l:nat -> #n1:tree_size l -> #n2:tree_size l -> #leaf_t:Type -> #node_t:Type -> dir:direction -> (tree l n1 leaf_t node_t & tree l n2 leaf_t node_t) -> (tree l (if dir = Left then n1 else n2) leaf_t node_t & tree l (if dir = Left then n2 else n1) leaf_t node_t)
-let order_subtrees #l #n1 #n2 #leaf_t #node_t dir (left,right) =
+let child_index (l:pos) (i:leaf_index l) : (direction & leaf_index (l-1)) =
+  if i < pow2 (l - 1) then (Left, i) else (Right, i-pow2 (l-1))
+
+val order_subtrees: #l:nat -> #leaf_t:Type -> #node_t:Type -> dir:direction -> (tree l leaf_t node_t & tree l leaf_t node_t) -> (tree l leaf_t node_t & tree l leaf_t node_t)
+let order_subtrees #l #leaf_t #node_t dir (left,right) =
   if dir = Left then (left,right) else (right,left)
 
-val get_leaf_list: #l:nat -> #n:tree_size l -> #leaf_t:Type -> #node_t:Type -> tree l n leaf_t node_t -> Pure (list leaf_t) (requires True) (fun res -> List.Tot.length res == n)
-let rec get_leaf_list #l #n #leaf_t #node_t t =
+val get_leaf_list: #l:nat -> #leaf_t:Type -> #node_t:Type -> tree l leaf_t node_t -> Pure (list leaf_t) (requires True) (fun res -> List.Tot.length res == pow2 l)
+let rec get_leaf_list #l #leaf_t #node_t t =
   let open FStar.List.Tot in
   match t with
   | TLeaf data -> [data]
-  | TSkip _ t' -> get_leaf_list t'
   | TNode _ left right ->
     (get_leaf_list left) @ (get_leaf_list right)
 
-val get_leaf: #l:nat -> #n:tree_size l -> #leaf_t:Type -> #node_t:Type -> tree l n leaf_t node_t -> leaf_index n -> leaf_t
-let rec get_leaf #l #n #leaf_t #node_t t i =
+val get_leaf: #l:nat -> #leaf_t:Type -> #node_t:Type -> tree l leaf_t node_t -> leaf_index l -> leaf_t
+let get_leaf #l #leaf_t #node_t t i =
   List.Tot.index (get_leaf_list t) i
 
-val print_tree: #l:nat -> #n:tree_size l -> #leaf_t:Type -> #node_t:Type -> (leaf_t -> string) -> (node_t -> string) -> tree l n leaf_t node_t -> string
-let rec print_tree #l #n #leaf_t #node_t print_leaf print_node t =
+val print_tree: #l:nat -> #leaf_t:Type -> #node_t:Type -> (leaf_t -> string) -> (node_t -> string) -> tree l leaf_t node_t -> string
+let rec print_tree #l #leaf_t #node_t print_leaf print_node t =
   match t with
   | TLeaf data -> print_leaf data
-  | TSkip _ t' -> print_tree print_leaf print_node t'
   | TNode data left right ->
     "(" ^ print_tree print_leaf print_node left ^ ") " ^ print_node data ^ " (" ^ print_tree print_leaf print_node right ^ ")"
