fstar/MLS.TreeSync.ParentHash.fst
@@ -28,25 +28,8 @@ let get_encryption_key_from_content #bytes #bl content =
     (parse (treekem_content_nt bytes) content);
   return content.encryption_key
 
-val mk_full_blank_tree: #bytes:Type0 -> {|bytes_like bytes|} -> l:nat -> treesync bytes l (pow2 l)
-let rec mk_full_blank_tree #bytes #bl l =
-  if l = 0 then
-    TLeaf None
-  else
-    TNode None (mk_full_blank_tree (l-1)) (mk_full_blank_tree (l-1))
-
-val fully_extend: #bytes:Type0 -> {|bytes_like bytes|} -> #l:nat -> #n:tree_size l -> treesync bytes l n -> treesync bytes l (pow2 l)
-let rec fully_extend #bytes #bl #l #n t =
-  match t with
-  | TLeaf olp ->
-    TLeaf olp
-  | TSkip _ t' ->
-    TNode None (fully_extend t') (mk_full_blank_tree _)
-  | TNode onp left right ->
-    TNode onp left (fully_extend right)
-
-val un_add: #bytes:Type0 -> {|bytes_like bytes|} -> #l:nat -> #n:tree_size l -> treesync bytes l n -> list nat -> nat -> treesync bytes l n
-let rec un_add #bytes #bl #l #n t leaves nb_left_leaves =
+val un_add: #bytes:Type0 -> {|bytes_like bytes|} -> #l:nat -> treesync bytes l -> list nat -> nat -> treesync bytes l
+let rec un_add #bytes #bl #l t leaves nb_left_leaves =
   match t with
   | TLeaf olp -> (
     if List.Tot.mem nb_left_leaves leaves then
@@ -54,8 +37,6 @@ let rec un_add #bytes #bl #l #n t leaves nb_left_leaves =
     else
       TLeaf olp
   )
-  | TSkip _ t' ->
-    TSkip _ (un_add t' leaves nb_left_leaves)
   | TNode onp left right ->
     let new_onp =
       match onp with
@@ -69,10 +50,10 @@ let rec un_add #bytes #bl #l #n t leaves nb_left_leaves =
     let new_right = un_add right leaves (nb_left_leaves + pow2 (l-1)) in
     TNode new_onp new_left new_right
 
-val compute_parent_hash_from_sibling: #bytes:Type0 -> {|crypto_bytes bytes|} -> #ls:nat -> #ns:tree_size ls -> node_package_t bytes -> nat -> treesync bytes ls ns -> result (lbytes bytes (hash_length #bytes))
-let compute_parent_hash_from_sibling #bytes #cb #ls #ns root_np nb_left_leaves_sibling sibling =
+val compute_parent_hash_from_sibling: #bytes:Type0 -> {|crypto_bytes bytes|} -> #ls:nat -> node_package_t bytes -> nat -> treesync bytes ls -> result (lbytes bytes (hash_length #bytes))
+let compute_parent_hash_from_sibling #bytes #cb #ls root_np nb_left_leaves_sibling sibling =
   encryption_key <-- get_encryption_key_from_content root_np.content.content;
-  original_sibling_tree_hash <-- tree_hash (fully_extend (un_add sibling root_np.unmerged_leaves nb_left_leaves_sibling));
+  original_sibling_tree_hash <-- tree_hash (un_add sibling root_np.unmerged_leaves nb_left_leaves_sibling);
   if not (length root_np.parent_hash < pow2 30) then
     internal_failure "compute_parent_hash_from_sibling: parent_hash too long"
   else (
@@ -83,8 +64,8 @@ let compute_parent_hash_from_sibling #bytes #cb #ls #ns root_np nb_left_leaves_s
     }))
   )
 
-val compute_parent_hash_from_dir: #bytes:Type0 -> {|crypto_bytes bytes|} -> #l:nat -> #n:tree_size l -> nat -> treesync bytes l n -> direction -> result (lbytes bytes (hash_length #bytes))
-let compute_parent_hash_from_dir #bytes #cb #l #n nb_left_leaves root dir =
+val compute_parent_hash_from_dir: #bytes:Type0 -> {|crypto_bytes bytes|} -> #l:nat -> nat -> treesync bytes l -> direction -> result (lbytes bytes (hash_length #bytes))
+let compute_parent_hash_from_dir #bytes #cb #l nb_left_leaves root dir =
   match root with
   | TNode (Some root_np) left right ->
     let (_, sibling) = order_subtrees dir (left, right) in
