fstar/MLS.TreeSync.fst
@@ -7,19 +7,18 @@ open MLS.TreeSync.Types
 
 (*** Tree creation ***)
 
-val create_tree: #bytes:Type0 -> {|bytes_like bytes|} -> leaf_package_t bytes -> treesync bytes 0 1
+val create_tree: #bytes:Type0 -> {|bytes_like bytes|} -> leaf_package_t bytes -> treesync bytes 0
 let create_tree lp =
   TLeaf (Some lp)
 
 (*** Tree operations ***)
 
-val tree_add: #bytes:Type0 -> {|bytes_like bytes|} -> #l:nat -> #n:tree_size l -> treesync bytes l n -> nat -> i:leaf_index n -> leaf_package_t bytes -> treesync bytes l n
-let rec tree_add #bytes #bl #l #n t original_i i lp =
+val tree_add: #bytes:Type0 -> {|bytes_like bytes|} -> #l:nat -> treesync bytes l -> nat -> i:leaf_index l -> leaf_package_t bytes -> treesync bytes l
+let rec tree_add #bytes #bl #l t original_i i lp =
   match t with
   | TLeaf _ -> TLeaf (Some lp)
-  | TSkip _ t' -> TSkip _ (tree_add t' original_i i lp)
   | TNode opt_content left right -> (
-    let (|dir, new_i|) = child_index l i in
+    let (dir, new_i) = child_index l i in
     let new_opt_content =
       match opt_content with
       | None -> None
@@ -32,85 +31,58 @@ let rec tree_add #bytes #bl #l #n t original_i i lp =
     else TNode new_opt_content left (tree_add right original_i new_i lp)
    )
 
-val tree_blank_path: #bytes:Type0 -> {|bytes_like bytes|} -> #l:nat -> #n:tree_size l -> treesync bytes l n -> i:leaf_index n -> option (leaf_package_t bytes) -> treesync bytes l n
-let rec tree_blank_path #bytes #bl #l #n t i opt_lp =
+val tree_blank_path: #bytes:Type0 -> {|bytes_like bytes|} -> #l:nat -> treesync bytes l -> i:leaf_index l -> option (leaf_package_t bytes) -> treesync bytes l
+let rec tree_blank_path #bytes #bl #l t i opt_lp =
   match t with
   | TLeaf _ -> TLeaf opt_lp
-  | TSkip _ t' -> TSkip _ (tree_blank_path t' i opt_lp)
   | TNode opt_node_content left right -> (
-    let (|dir, new_i|) = child_index l i in
+    let (dir, new_i) = child_index l i in
     if dir = Left
     then TNode None (tree_blank_path left new_i opt_lp) right
     else TNode None left (tree_blank_path right new_i opt_lp)
   )
 
-val tree_update: #bytes:Type0 -> {|bytes_like bytes|} -> #l:nat -> #n:tree_size l -> treesync bytes l n -> i:leaf_index n -> leaf_package_t bytes -> treesync bytes l n
-let tree_update #bytes #bl #l #n t i lp =
+val tree_update: #bytes:Type0 -> {|bytes_like bytes|} -> #l:nat -> treesync bytes l -> i:leaf_index l -> leaf_package_t bytes -> treesync bytes l
+let tree_update #bytes #bl #l t i lp =
   tree_blank_path t i (Some lp)
 
-val tree_remove: #bytes:Type0 -> {|bytes_like bytes|} -> #l:nat -> #n:tree_size l -> treesync bytes l n -> i:leaf_index n -> treesync bytes l n
-let tree_remove #bytes #bl #l #n t i =
+val tree_remove: #bytes:Type0 -> {|bytes_like bytes|} -> #l:nat -> treesync bytes l -> i:leaf_index l -> treesync bytes l
+let tree_remove #bytes #bl #l t i =
   tree_blank_path t i None
 
-val apply_path: #bytes:Type0 -> {|bytes_like bytes|} -> #l:nat -> #n:tree_size l -> #i:leaf_index n -> treesync bytes l n -> pathsync bytes l n i -> treesync bytes l n
-let rec apply_path #bytes #bl #l #n #i t p =
+val apply_path: #bytes:Type0 -> {|bytes_like bytes|} -> #l:nat -> treesync bytes l -> pathsync bytes l -> leaf_index l -> treesync bytes l
+let rec apply_path #bytes #bl #l t p i =
   match t,p with
   | TLeaf _, PLeaf m' -> TLeaf m'
-  | TSkip _ t', PSkip _ p' -> TSkip _ (apply_path t' p')
   | TNode _ left right, PNode onp next ->
-     let (|dir,_|) = child_index l i in
+     let (dir,new_i) = child_index l i in
      if dir = Left
-     then TNode onp (apply_path left next) right
-     else TNode onp left (apply_path right next)
+     then TNode onp (apply_path left next new_i) right
+     else TNode onp left (apply_path right next new_i)
 
 
 (*** Tree extension / truncation ***)
 
-val is_tree_empty: #bytes:Type0 -> {|bytes_like bytes|} -> #l:nat -> #n:tree_size l -> treesync bytes l n -> bool
-let rec is_tree_empty #bytes #bl #l #n t =
+val is_tree_empty: #bytes:Type0 -> {|bytes_like bytes|} -> #l:nat -> treesync bytes l -> bool
+let rec is_tree_empty #bytes #bl #l t =
   match t with
   | TNode _ left right ->
     is_tree_empty left && is_tree_empty right
-  | TSkip _ t' -> is_tree_empty t'
   | TLeaf (Some _) -> false
   | TLeaf None -> true
 
-val add_skips: #bytes:Type0 -> {|bytes_like bytes|} -> #l:nat -> #n:tree_size l -> treesync bytes l n -> (n_res:tree_size l{n_res <= n} & treesync bytes l n_res)
-let rec add_skips #bytes #bl #l #n t =
-  match t with
-  | TNode data left right ->
-    if is_tree_empty right && None? data then (
-      let (|n_res, left_res|) = add_skips left in
-      (|n_res, TSkip _ left_res|)
-    ) else (
-      let (|n_right_res, right_res|) = add_skips right in
-      (|pow2 (l-1) + n_right_res, TNode data left right_res|)
-    )
-  | TSkip _ t' ->
-    let (|n_res, t_res|) = add_skips t' in
-    (|n_res, TSkip () t_res|)
-  | TLeaf _ -> (|n, t|)
-
-val remove_root_skip: #bytes:Type0 -> {|bytes_like bytes|} -> #l:nat -> #n:tree_size l -> treesync bytes l n -> (l_res:nat{l_res <= l} & n_res:tree_size l_res{n_res == n} & treesync bytes l_res n_res)
-let rec remove_root_skip #bytes #bl #l #n t =
-  match t with
-  | TNode _ _ _ -> (|l, n, t|)
-  | TSkip _ t' ->
-    //`let` necessary for F* to see that l_res <= l-1 implies l_res <= l
-    let (|l_res, n_res, t_res|) = remove_root_skip t' in
-    (|l_res, n_res, t_res|)
-  | TLeaf _ -> (|l, n, t|)
-
-val canonicalize_tree: #bytes:Type0 -> {|bytes_like bytes|} -> #l:nat -> #n:tree_size l -> treesync bytes l n -> (l_res:nat{l_res <= l} & n_res:tree_size l_res{n_res <= n} & treesync bytes l_res n_res)
-let canonicalize_tree #bytes #bl #l #n t0 =
-  let (|_, t1|) = add_skips t0 in
-  let (|l_res, n_res, t_res|) = remove_root_skip t1 in
-  (|l_res, n_res, t_res|)
+val canonicalize_tree: #bytes:Type0 -> {|bytes_like bytes|} -> #l:nat -> treesync bytes l -> (l_res:nat{l_res <= l} & treesync bytes l_res)
+let canonicalize_tree #bytes #bl #l t0 =
+  match t0 with
+  | TLeaf _ -> (|_, t0|)
+  | TNode _ left right ->
+    if is_tree_empty right then (|_, left|)
+    else (|_, t0|)
 
 // Helper functions to add leaf / extend the tree
 
-val find_empty_leaf: #bytes:Type0 -> {|bytes_like bytes|} -> #l:nat -> #n:tree_size l -> treesync bytes l n -> option (leaf_index n)
-let rec find_empty_leaf #bytes #bl #l #n t =
+val find_empty_leaf: #bytes:Type0 -> {|bytes_like bytes|} -> #l:nat -> treesync bytes l -> option (leaf_index l)
+let rec find_empty_leaf #bytes #bl #l t =
   match t with
   | TNode _ left right -> (
     match find_empty_leaf left, find_empty_leaf right with
@@ -118,32 +90,17 @@ let rec find_empty_leaf #bytes #bl #l #n t =
     | None, Some x -> Some ((pow2 (l-1)) + x)
     | None, None -> None
   )
-  | TSkip _ t' -> find_empty_leaf t'
   | TLeaf (Some _) -> None
   | TLeaf None -> Some 0
 
-val mk_one_leaf_tree: #bytes:Type0 -> {|bytes_like bytes|} -> l:nat -> Pure (treesync bytes l 1) (requires True) (fun res -> Some? (find_empty_leaf res))
-let rec mk_one_leaf_tree #bytes #bl l =
-  if l = 0 then
-    TLeaf None
-  else
-    TSkip () (mk_one_leaf_tree (l-1))
+val mk_blank_tree: #bytes:Type0 -> {|bytes_like bytes|} -> l:nat -> Pure (treesync bytes l) (requires True) (ensures fun res -> Some? (find_empty_leaf res))
+let rec mk_blank_tree #bytes #bl l =
+  if l = 0 then TLeaf None
+  else TNode None (mk_blank_tree (l-1)) (mk_blank_tree (l-1))
 
-val add_one_leaf: #bytes:Type0 -> {|bytes_like bytes|} -> #l:nat -> #n:tree_size l{n <> pow2 l} -> treesync bytes l n -> Pure (treesync bytes l (n+1)) (requires True) (fun res -> Some? (find_empty_leaf res))
-let rec add_one_leaf #bytes #bl #l #n t =
-  match t with
-  | TNode np left right -> (
-    TNode np left (add_one_leaf right)
-  )
-  | TSkip _ t' ->
-    if n = pow2 (l-1) then
-      TNode None t' (mk_one_leaf_tree (l-1))
-    else
-      TSkip () (add_one_leaf t')
-
-val add_one_level: #bytes:Type0 -> {|bytes_like bytes|} -> #l:nat -> treesync bytes l (pow2 l) -> Pure (treesync bytes (l+1) ((pow2 l)+1)) (requires True) (fun res -> Some? (find_empty_leaf res))
+val add_one_level: #bytes:Type0 -> {|bytes_like bytes|} -> #l:nat -> treesync bytes l -> Pure (treesync bytes (l+1)) (requires True) (fun res -> Some? (find_empty_leaf res))
 let add_one_level #bytes #bl #l t =
-  TNode None t (mk_one_leaf_tree l)
+  TNode None t (mk_blank_tree l)
 
 (*** Higher-level API ***)
 
@@ -154,13 +111,12 @@ open MLS.Result
 
 val create: #bytes:Type0 -> {|bytes_like bytes|} -> gid:bytes -> leaf_package_t bytes -> state_t bytes
 let create #bytes #bl gid lp =
-  mk_initial_state gid 0 1 (create_tree lp)
+  mk_initial_state gid 0 (create_tree lp)
 
-val state_update_tree: #bytes:Type0 -> {|bytes_like bytes|} -> #l:level_n -> #n:tree_size l -> state_t bytes -> treesync bytes l n -> state_t bytes
-let state_update_tree #bytes #bl #l #n st new_tree =
+val state_update_tree: #bytes:Type0 -> {|bytes_like bytes|} -> #l:level_n -> state_t bytes -> treesync bytes l -> state_t bytes
+let state_update_tree #bytes #bl #l st new_tree =
   ({ st with
     levels = l;
-    treesize = n;
     version = st.version + 1;
     tree = new_tree;
     //transcript = Seq.snoc st.transcript op //TODO
@@ -182,14 +138,7 @@ let add #bytes #bl st kp =
   | Some i ->
     return (state_update_tree st (tree_add st.tree i i lp), (i <: nat))
   | None ->
-    let new_l = if st.treesize = pow2 st.levels then st.levels+1 else st.levels in
-    let new_n = st.treesize+1 in
-    let augmented_tree: treesync bytes new_l new_n =
-      if st.treesize = pow2 st.levels then
-        add_one_level st.tree
-      else
-        add_one_leaf st.tree
-    in
+    let augmented_tree = add_one_level st.tree in
     let i = Some?.v (find_empty_leaf augmented_tree) in
     return (state_update_tree st (tree_add augmented_tree i i lp), i)
 
@@ -200,5 +149,5 @@ let update #bytes #bl st lp i =
 val remove: #bytes:Type0 -> {|bytes_like bytes|} -> st:state_t bytes -> i:index_t st -> state_t bytes
 let remove #bytes #bl st i =
   let blanked_tree = (tree_remove st.tree i) in
-  let (|_, _, reduced_tree|) = canonicalize_tree blanked_tree in
+  let (|_, reduced_tree|) = canonicalize_tree blanked_tree in
   state_update_tree st reduced_tree
